Work done

Sort.v
@@ -7,6 +7,15 @@ Require Import SfLib.
 Notation "[ ]" := nil.
 Notation "[ x , .. , y ]" := (cons x .. (cons y nil) ..).
 
+Theorem ble_nat_refl: forall m, ble_nat m m = true.
+Proof.
+  intros. induction m as [| m'].
+  Case "m = 0".
+  reflexivity.
+  Case "m = S m'".
+  apply IHm'.
+Qed.
+
 Theorem ble_nat_i: forall n m, n <= m -> ble_nat n m = true.
 Proof.
 induction n as [|n']; intros; simpl; auto.
@@ -58,24 +67,104 @@ Qed.
 
 (* Prove an auxiliary lemma insert_perm, useful for proving sort_perm.
   You may want to get into the proof of sort_perm first, to see what you'll need.  *)
-(* FILL IN HERE *)
+Theorem insert_perm_l: forall l i, Permutation (i::l) (insert i l).
+Proof.
+  intros. induction l as [| x xs].
+  reflexivity.
+  simpl. destruct (ble_nat i x).
+    reflexivity.
+    rewrite <- IHxs. apply perm_swap.
+Qed.
+
+Theorem insert_perm: forall l l' i,
+  Permutation l l' -> Permutation (i::l) (insert i l').
+Proof.
+  intros. destruct l' as [| y ys].
+    simpl. apply perm_skip. apply H.
+    destruct l.
+      apply Permutation_nil in H. rewrite H. reflexivity.
+      rewrite H. apply insert_perm_l.
+Qed.
 
 (** **** Exercise: 3 stars *)
 (* Now prove the main theorem. *)
 Theorem sort_perm: forall l, Permutation l (sort l).
-(* FILL IN HERE *) Admitted.
+Proof.
+  intros. induction l as [| x xs].
+    reflexivity.
+    apply insert_perm. assumption.
+Qed.
 (** [] *)
 
 (** **** Exercise: 3 stars *)
 (* Define an inductive predicate "sorted" that tells whether a list of nats is in nondecreasing order.
    Then prove that "sort" produces a sorted list.
 *)
-Inductive sorted: list nat -> Prop := 
- (* FILL IN HERE *)
-.
+Inductive sorted: list nat -> Prop :=
+  | sorted_nil : sorted []
+  | sorted_cons1 x : sorted [x]
+  | sorted_cons x y l : sorted (y::l) -> ble_nat x y = true -> sorted (x::y::l).
+
+Theorem sorted_zero: forall l, sorted l -> sorted (0 :: l).
+Proof.
+  intros. induction l as [| x xs].
+    apply sorted_cons1.
+    inversion H.
+      apply sorted_cons.
+        apply sorted_cons1.
+        reflexivity.
+      rewrite H1.
+      apply sorted_cons.
+        apply H.
+        reflexivity.
+Qed.
+
+Theorem sorted_rest: forall l i, sorted (i :: l) -> sorted l.
+Proof.
+  intros. induction l as [| x xs].
+    apply sorted_nil.
+    inversion H. apply H2.
+Qed.
+
+Theorem ble_nat_flip: forall i x, ble_nat i x = false -> ble_nat x i = true.
+Proof.
+  intros. generalize dependent x.
+  induction i as [| i'].
+  Case "i = 0".
+  destruct x.
+    reflexivity.
+    intros. inversion H.
+  Case "i = S i'".
+  induction x.
+    reflexivity.
+    intros. simpl. apply IHi'.
+    inversion H. reflexivity.
+Qed.
+
+Theorem insert_sorted: forall l i, sorted l -> sorted (insert i l).
+Proof.
+  intros.
+  induction l as [| x xs].
+    simpl. constructor.
+    simpl. destruct (ble_nat i x) eqn:Heqe.
+      constructor. assumption. assumption.
+      inversion H; subst.
+        simpl. constructor. constructor.
+          apply ble_nat_flip. apply Heqe.
+        simpl. simpl in IHxs.
+        simpl. destruct (ble_nat i y) eqn:Heqe2.
+          constructor.
+          constructor. apply H2. apply Heqe2.
+          apply ble_nat_flip. apply Heqe.
+          constructor. apply IHxs. apply H2. apply H3.
+Qed.
 
 (* You may want to first prove an auxiliary lemma about inserting an element
    into a sorted list.  *)
 Theorem sort_sorted: forall l, sorted (sort l).
-(* FILL IN HERE *) Admitted.
+Proof.
+  intros. induction l as [| x xs].
+    apply sorted_nil.
+    apply insert_sorted. apply IHxs.
+Qed.
 (** [] *)
